theories/Logic/inverse_ug_l.v
@@ -25,11 +25,15 @@ match P, S with
 
 | equal v1 v2, _ => P
 
-| loop_head OC1 OC2 gamma delta sig P_Target, _ => loop_head OC1 OC2 (ug_left_inv_batch gamma A i S) delta sig (ptree_ug_l_inv_fit P_Target A i (list_filter S (sublist_filter form_eq_dec (map (fun lambda => sig_subst lambda (sig_generalise sig)) (ptree_left P_Target)) gamma)))
+| loop_head OC gamma delta alpha P_Target, _ => loop_head OC (ug_left_inv_batch gamma A i S) delta alpha (REC P_Target S)
 
-| @con_l OC gamma delta phi v1 v2 alpha P', s1 :: s2 :: S' => @con_l OC (ug_left_inv_batch gamma A i S') delta (ug_left_inv_formula phi A i s2) v1 v2 alpha (REC P' (s1 :: s2 :: s2 :: S'))
+| @con_l OC gamma delta phi alpha P', s :: S' => @con_l OC (ug_left_inv_batch gamma A i S') delta (ug_left_inv_formula phi A i s) alpha (REC P' (s :: s :: S'))
 
 | @con_r OC gamma delta phi alpha P', _ => @con_r OC (ptree_left (REC P' S)) delta phi alpha (REC P' S)
+
+| @sub_l OC gamma delta phi v1 v2 alpha P', s1 :: s2 :: S' => @sub_l OC (ug_left_inv_batch gamma A i S') delta (ug_left_inv_formula phi A i s2) v1 v2 alpha (REC P' (s1 :: s2 :: S'))
+
+| @sub_r OC gamma delta phi v1 v2 alpha P', s :: S' => @sub_r OC (ug_left_inv_batch gamma A i S') delta phi v1 v2 alpha (REC P' (s :: S'))
 
 | @refl OC gamma delta v alpha P', _ => @refl OC (ug_left_inv_batch gamma A i S) delta v alpha (ptree_ug_l_inv_fit P' A i (false :: S))
 
@@ -81,13 +85,14 @@ Proof. intros P A v S EQ. unfold ptree_ug_l_inv. rewrite EQ. reflexivity. Qed.
 Lemma ptree_ug_l_inv_left :
     forall (P : ptree) (A : formula) (v : ivar),
         struct_valid P ->
-            forall (S : subst_ind),
-                ptree_left (ptree_ug_l_inv P A v S) =
-                    (ug_left_inv_batch (ptree_left P) A v S).
+            weak_formula A = false ->
+                forall (S : subst_ind),
+                    ptree_left (ptree_ug_l_inv P A v S) =
+                        (ug_left_inv_batch (ptree_left P) A v S).
 Proof.
 intros P A v.
 induction P;
-try intros PSV S;
+try intros PSV WF S;
 unfold ptree_ug_l_inv;
 unfold ug_left_inv_batch, batch_sub;
 case nat_eqb eqn:EQ;
@@ -98,15 +103,16 @@ unfold ptree_left in EQ;
 fold ptree_left in EQ.
 
 1-3 : destruct PSV.
-4 : destruct PSV as [[[PSV [PG_app PD_app]] Psig] PLoop].
-5-11 : destruct PSV as [[[[[PSV [PG_app PD_app]] PG] PD] POC] PDeg].
-12 : destruct PSV as [[[[[[[PSV [PG_app PD_app]] PG] PD] KNING] KNIND] [KIN POC]] PDeg].
-13-14 : destruct PSV as [[[[[PSV [PG_app PD_app]] PG] PD] POC] PDeg].
-15 : destruct PSV as [[[[[[PSV [PG_app PD_app]] PG] PD] POC] POC_rel] PDeg].
-16 : destruct PSV as [[[[[[PSV [PG_app PD_app]] PG] PD] [NEW [KIN POC]]] [NING NIND]] PDeg].
-17 : destruct PSV as [[[[[[[[[[P1SV P2SV] [PG_app PD_app]] P1G] P1D] P1OC] P2G] P2D] P2OC] PDeg1] PDeg2].
-18 : destruct PSV as [[[[[PSV [PG_app PD_app]] PG] PD] POC] PDeg].
-19 : destruct PSV as [[[[[[[[[[P1SV P2SV] [PG_app PD_app]] P1G] P1D] P1OC] P2G] P2D] P2OC] PDeg1] PDeg2].
+4 : destruct PSV as [[[PSV [PG_app PD_app]] [PBot | [[[[PRec PG] PD] POC] PDeg]]] PWF].
+6-12 : destruct PSV as [[[[[PSV [PG_app PD_app]] PG] PD] POC] PDeg].
+13-14 : destruct PSV as [[[[[[PSV [PG_app PD_app]] PG] PD] POC] PDeg] PWF].
+15 : destruct PSV as [[[[[[[PSV [PG_app PD_app]] PG] PD] KNING] KNIND] [KIN POC]] PDeg].
+16-17 : destruct PSV as [[[[[PSV [PG_app PD_app]] PG] PD] POC] PDeg].
+18 : destruct PSV as [[[[[[PSV [PG_app PD_app]] PG] PD] POC] POC_rel] PDeg].
+19 : destruct PSV as [[[[[[PSV [PG_app PD_app]] PG] PD] [NEW [KIN POC]]] [NING NIND]] PDeg].
+20 : destruct PSV as [[[[[[[[[[P1SV P2SV] [PG_app PD_app]] P1G] P1D] P1OC] P2G] P2D] P2OC] PDeg1] PDeg2].
+21 : destruct PSV as [[[[[PSV [PG_app PD_app]] PG] PD] POC] PDeg].
+22 : destruct PSV as [[[[[[[[[[P1SV P2SV] [PG_app PD_app]] P1G] P1D] P1OC] P2G] P2D] P2OC] PDeg1] PDeg2].
 
 all : subst;
       unfold ptree_left at 2;
@@ -114,18 +120,17 @@ all : subst;
       unfold batch_sub_fit;
       fold @batch_sub_fit.
 
-6,9,11,12,14,16 : rewrite (batch_sub_fit_true EQ);
-                  rewrite (ptree_ug_l_inv_fit_true EQ);
-                  apply (IHP PSV).
+7,12,14,15,17,19 :  rewrite (batch_sub_fit_true EQ);
+                    rewrite (ptree_ug_l_inv_fit_true EQ);
+                    apply (IHP PSV WF).
 
 1-3 : destruct S;
       reflexivity.
 
-- rewrite (batch_sub_fit_true EQ).
-  reflexivity.
+all : try rewrite (batch_sub_fit_true EQ);
+      try reflexivity.
 
-- destruct S as [ | b1 [ | b2 S]].
-  inversion EQ.
+- destruct S as [ | b S];
   inversion EQ.
   rewrite batch_sub_fit_true, ptree_ug_l_inv_fit_true.
   reflexivity.
@@ -133,24 +138,37 @@ all : subst;
   apply EQ.
   apply EQ.
 
-- rewrite (batch_sub_fit_true EQ).
+- destruct S as [ | b1 [ | b2 S]].
+  1,2 : inversion EQ.
+  unfold ptree_left.
+  unfold formula_sub at 1.
+  unfold form_eqb, ug_left_inv_formula, ug_left_inv_batch.
+  rewrite batch_sub_fit_true.
+  2 : apply EQ.
+  unfold form_equiv at 1.
+  rewrite (form_sub_sub0_comm _ _ _ _ _ WF).
   reflexivity.
+
+- destruct S as [ | b S].
+  inversion EQ.
+  rewrite batch_sub_fit_true.
+  reflexivity.
+  apply EQ.
 
 - unfold ptree_left at 1.
   fold (ptree_left (ptree_ug_l_inv_fit P A v (unbury S n))).
-  rewrite batch_sub_fit_true, ptree_ug_l_inv_fit_true, <- batch_bury_comm, (IHP PSV).
+  rewrite ptree_ug_l_inv_fit_true, <- batch_bury_comm, (IHP PSV WF).
   reflexivity.
   rewrite bury_length, <- (@bury_unbury _ S n), bury_length in EQ.
-  apply EQ.
   apply EQ.
 
 - destruct S as [ | b S].
   inversion EQ.
   unfold ptree_left at 1 2.
   fold (ptree_left P).
-  unfold batch_sub_fit;
-  fold batch_sub_fit.  
-  rewrite batch_sub_fit_true.
+  unfold batch_sub, batch_sub_fit;
+  fold batch_sub_fit.
+  rewrite batch_sub_fit_true, EQ.
   reflexivity.
   apply EQ.
 
@@ -163,21 +181,35 @@ all : subst;
   + apply and_bool_prop in EQ' as [EQ1 EQ2].
     apply form_eqb_eq in EQ2.
     subst.
-    rewrite ptree_ug_l_inv_fit_true, (IHP PSV), PG.
+    rewrite ptree_ug_l_inv_fit_true, (IHP PSV WF), PG.
     unfold ug_left_inv_batch, batch_sub, batch_sub_fit at 1;
     fold batch_sub_fit.
     unfold length in *;
     fold (@length formula) (@length bool) in *.
     rewrite EQ, formula_sub_false.
+    apply nat_eqb_eq in EQ1.
+    subst.
+    rewrite form_equiv_refl.
     reflexivity.
     rewrite PG.
     apply EQ.
   + unfold ptree_left.
     rewrite batch_sub_fit_true.
+    apply and_bool_prop in EQ' as [EQ1 EQ2].
+    apply nat_eqb_eq in EQ1.
+    apply form_eqb_eq in EQ2.
+    subst.
+    rewrite form_equiv_refl.
     reflexivity.
     apply EQ.
   + unfold ptree_left.
     rewrite batch_sub_fit_true.
+    unfold form_equiv;
+    fold form_equiv.
+    case (nat_eqb v0 v) eqn:EQN;
+    try apply nat_eqb_eq in EQN;
+    subst;
+    rewrite (not_weak_equiv_eqb _ _ WF), EQ';
     reflexivity.
     apply EQ.
 
@@ -192,18 +224,9 @@ all : subst;
   inversion EQ.
   unfold ptree_left at 1 2;
   fold (ptree_left P2).
-  unfold batch_sub_fit;
+  unfold batch_sub, batch_sub_fit;
   fold batch_sub_fit.
-  rewrite batch_sub_fit_true.
-  reflexivity.
-  apply EQ.
-
-- rewrite (batch_sub_fit_true EQ).
-  reflexivity.
-
-- unfold ptree_left at 1.
-  fold (ptree_left P1).
-  rewrite batch_sub_fit_true.
+  rewrite batch_sub_fit_true, EQ.
   reflexivity.
   apply EQ.
 Qed.
@@ -222,15 +245,16 @@ unfold ptree_ug_l_inv;
 unfold ug_left_inv_batch, batch_sub.
 
 1-3 : destruct PSV.
-4 : destruct PSV as [[[PSV [PG_app PD_app]] Psig] PLoop].
-5-11 : destruct PSV as [[[[[PSV [PG_app PD_app]] PG] PD] POC] PDeg].
-12 : destruct PSV as [[[[[[[PSV [PG_app PD_app]] PG] PD] KNING] KNIND] [KIN POC]] PDeg].
-13-14 : destruct PSV as [[[[[PSV [PG_app PD_app]] PG] PD] POC] PDeg].
-15 : destruct PSV as [[[[[[PSV [PG_app PD_app]] PG] PD] POC] POC_rel] PDeg].
-16 : destruct PSV as [[[[[[PSV [PG_app PD_app]] PG] PD] [NEW [KIN POC]]] [NING NIND]] PDeg].
-17 : destruct PSV as [[[[[[[[[[P1SV P2SV] [PG_app PD_app]] P1G] P1D] P1OC] P2G] P2D] P2OC] PDeg1] PDeg2].
-18 : destruct PSV as [[[[[PSV [PG_app PD_app]] PG] PD] POC] PDeg].
-19 : destruct PSV as [[[[[[[[[[P1SV P2SV] [PG_app PD_app]] P1G] P1D] P1OC] P2G] P2D] P2OC] PDeg1] PDeg2].
+4 : destruct PSV as [[[PSV [PG_app PD_app]] [PBot | [[[[PRec PG] PD] POC] PDeg]]] PWF].
+6-12 : destruct PSV as [[[[[PSV [PG_app PD_app]] PG] PD] POC] PDeg].
+13-14 : destruct PSV as [[[[[[PSV [PG_app PD_app]] PG] PD] POC] PDeg] PWF].
+15 : destruct PSV as [[[[[[[PSV [PG_app PD_app]] PG] PD] KNING] KNIND] [KIN POC]] PDeg].
+16-17 : destruct PSV as [[[[[PSV [PG_app PD_app]] PG] PD] POC] PDeg].
+18 : destruct PSV as [[[[[[PSV [PG_app PD_app]] PG] PD] POC] POC_rel] PDeg].
+19 : destruct PSV as [[[[[[PSV [PG_app PD_app]] PG] PD] [NEW [KIN POC]]] [NING NIND]] PDeg].
+20 : destruct PSV as [[[[[[[[[[P1SV P2SV] [PG_app PD_app]] P1G] P1D] P1OC] P2G] P2D] P2OC] PDeg1] PDeg2].
+21 : destruct PSV as [[[[[PSV [PG_app PD_app]] PG] PD] POC] PDeg].
+22 : destruct PSV as [[[[[[[[[[P1SV P2SV] [PG_app PD_app]] P1G] P1D] P1OC] P2G] P2D] P2OC] PDeg1] PDeg2].
 
 all : subst; 
       case nat_eqb eqn:EQ;
@@ -240,13 +264,11 @@ all : subst;
       unfold ptree_left in EQ;
       fold ptree_left in EQ.
 
-2,4,5 : destruct S as [ | b S];
+1,3,4,6,7 : destruct S as [ | b S];
         inversion EQ;
         reflexivity.
 
-- destruct S as [ | b1 [ | b2 S]].
-  inversion EQ.
-  inversion EQ.
+- destruct S as [ | b1 [ | b2 S]];
   reflexivity.
 
 - destruct S as [ | b S].
@@ -260,7 +282,6 @@ all : subst;
   rewrite PG.
   apply EQ.
 Qed.
-
 
 Lemma ptree_ug_l_inv_constraint :
     forall (P : ptree) (A : formula) (v : ivar),
@@ -276,15 +297,16 @@ unfold ptree_ug_l_inv;
 unfold ug_left_inv_batch, batch_sub.
 
 1-3 : destruct PSV.
-4 : destruct PSV as [[[PSV [PG_app PD_app]] Psig] PLoop].
-5-11 : destruct PSV as [[[[[PSV [PG_app PD_app]] PG] PD] POC] PDeg].
-12 : destruct PSV as [[[[[[[PSV [PG_app PD_app]] PG] PD] KNING] KNIND] [KIN POC]] PDeg].
-13-14 : destruct PSV as [[[[[PSV [PG_app PD_app]] PG] PD] POC] PDeg].
-15 : destruct PSV as [[[[[[PSV [PG_app PD_app]] PG] PD] POC] POC_rel] PDeg].
-16 : destruct PSV as [[[[[[PSV [PG_app PD_app]] PG] PD] [NEW [KIN POC]]] [NING NIND]] PDeg].
-17 : destruct PSV as [[[[[[[[[[P1SV P2SV] [PG_app PD_app]] P1G] P1D] P1OC] P2G] P2D] P2OC] PDeg1] PDeg2].
-18 : destruct PSV as [[[[[PSV [PG_app PD_app]] PG] PD] POC] PDeg].
-19 : destruct PSV as [[[[[[[[[[P1SV P2SV] [PG_app PD_app]] P1G] P1D] P1OC] P2G] P2D] P2OC] PDeg1] PDeg2].
+4 : destruct PSV as [[[PSV [PG_app PD_app]] [PBot | [[[[PRec PG] PD] POC] PDeg]]] PWF].
+6-12 : destruct PSV as [[[[[PSV [PG_app PD_app]] PG] PD] POC] PDeg].
+13-14 : destruct PSV as [[[[[[PSV [PG_app PD_app]] PG] PD] POC] PDeg] PWF].
+15 : destruct PSV as [[[[[[[PSV [PG_app PD_app]] PG] PD] KNING] KNIND] [KIN POC]] PDeg].
+16-17 : destruct PSV as [[[[[PSV [PG_app PD_app]] PG] PD] POC] PDeg].
+18 : destruct PSV as [[[[[[PSV [PG_app PD_app]] PG] PD] POC] POC_rel] PDeg].
+19 : destruct PSV as [[[[[[PSV [PG_app PD_app]] PG] PD] [NEW [KIN POC]]] [NING NIND]] PDeg].
+20 : destruct PSV as [[[[[[[[[[P1SV P2SV] [PG_app PD_app]] P1G] P1D] P1OC] P2G] P2D] P2OC] PDeg1] PDeg2].
+21 : destruct PSV as [[[[[PSV [PG_app PD_app]] PG] PD] POC] PDeg].
+22 : destruct PSV as [[[[[[[[[[P1SV P2SV] [PG_app PD_app]] P1G] P1D] P1OC] P2G] P2D] P2OC] PDeg1] PDeg2].
 
 all : subst; 
       case nat_eqb eqn:EQ;
@@ -294,13 +316,11 @@ all : subst;
       unfold ptree_left in EQ;
       fold ptree_left in EQ.
 
-2,4,5 : destruct S as [ | b S];
-        inversion EQ;
-        reflexivity.
+1,3,4,6,7 : destruct S as [ | b S];
+            inversion EQ;
+            reflexivity.
 
-- destruct S as [ | b1 [ | b2 S]].
-  inversion EQ.
-  inversion EQ.
+- destruct S as [ | b1 [ | b2 S]];
   reflexivity.
 
 - destruct S as [ | b S].
@@ -329,7 +349,113 @@ unfold ptree_ug_l_inv;
 unfold ug_left_inv_batch, batch_sub.
 
 1-3 : destruct PSV.
-4 : destruct PSV as [[[PSV [PG_app PD_app]] Psig] PLoop].
+4 : destruct PSV as [[[PSV [PG_app PD_app]] [PBot | [[[[PRec PG] PD] POC] PDeg]]] PWF].
+6-12 : destruct PSV as [[[[[PSV [PG_app PD_app]] PG] PD] POC] PDeg].
+13-14 : destruct PSV as [[[[[[PSV [PG_app PD_app]] PG] PD] POC] PDeg] PWF].
+15 : destruct PSV as [[[[[[[PSV [PG_app PD_app]] PG] PD] KNING] KNIND] [KIN POC]] PDeg].
+16-17 : destruct PSV as [[[[[PSV [PG_app PD_app]] PG] PD] POC] PDeg].
+18 : destruct PSV as [[[[[[PSV [PG_app PD_app]] PG] PD] POC] POC_rel] PDeg].
+19 : destruct PSV as [[[[[[PSV [PG_app PD_app]] PG] PD] [NEW [KIN POC]]] [NING NIND]] PDeg].
+20 : destruct PSV as [[[[[[[[[[P1SV P2SV] [PG_app PD_app]] P1G] P1D] P1OC] P2G] P2D] P2OC] PDeg1] PDeg2].
+21 : destruct PSV as [[[[[PSV [PG_app PD_app]] PG] PD] POC] PDeg].
+22 : destruct PSV as [[[[[[[[[[P1SV P2SV] [PG_app PD_app]] P1G] P1D] P1OC] P2G] P2D] P2OC] PDeg1] PDeg2].
+
+all : subst; 
+      case nat_eqb eqn:EQ;
+      try reflexivity;
+      unfold ptree_ug_l_inv_fit;
+      fold ptree_ug_l_inv_fit;
+      unfold ptree_left in EQ;
+      fold ptree_left in EQ.
+
+1,3,4,6,7 : destruct S as [ | b S];
+            inversion EQ;
+            reflexivity.
+
+- destruct S as [ | b1 [ | b2 S]];
+  reflexivity.
+
+- destruct S as [ | b S].
+  inversion EQ.
+  case (nat_eqb v0 v && form_eqb phi A).
+  case b.
+  2,3 : reflexivity.
+  unfold ptree_deg at 2.
+  rewrite ptree_ug_l_inv_fit_true.
+  apply (IHP PSV).
+  rewrite PG.
+  apply EQ.
+Qed.
+
+Lemma ug_l_formula_inv_vars :
+    forall (phi : formula) (A : formula) (v : ivar) (b : bool),
+        weak_formula A = false ->
+            vars_in (ug_left_inv_formula phi A v b) =
+                vars_in phi.
+Proof.
+intros phi A v b WF.
+unfold ug_left_inv_formula, formula_sub.
+case form_equiv eqn:EQF.
+destruct b.
+rewrite not_weak_equiv_eqb in EQF.
+apply form_eqb_eq in EQF.
+subst.
+all : try reflexivity.
+apply WF.
+Qed.
+
+Lemma ptree_ug_l_inv_vars :
+    forall (gamma : list formula) (A : formula) (v : ivar) (S : subst_ind),
+        weak_formula A = false ->
+            flat_map vars_in (ug_left_inv_batch gamma A v S) =
+                flat_map vars_in gamma.
+Proof.
+induction gamma;
+intros A v S WF;
+unfold ug_left_inv_batch, batch_sub, batch_sub_fit;
+fold batch_sub_fit;
+destruct S;
+unfold length, nat_eqb;
+fold (@length formula) (@length bool) nat_eqb.
+1-3 : reflexivity.
+case nat_eqb eqn:EQN.
+unfold flat_map;
+fold (flat_map vars_in).
+rewrite (batch_sub_fit_true EQN).
+fold (ug_left_inv_batch gamma A v S).
+rewrite (IHgamma _ _ _ WF).
+fold (ug_left_inv_formula a A v b).
+rewrite (ug_l_formula_inv_vars _ _ _ _ WF).
+reflexivity.
+reflexivity.
+Qed.
+
+Lemma ptree_ug_l_inv_bot :
+    forall (phi : formula) (v : ivar) (S : subst_ind),
+        ptree_ug_l_inv bot phi v S = bot.
+Proof.
+intros phi v S.
+unfold ptree_ug_l_inv, ptree_ug_l_inv_fit.
+case (nat_eqb);
+reflexivity.
+Qed.
+
+(*
+Lemma ptree_ug_l_inv_leaves :
+    forall (P : ptree) (A : formula) (v : ivar),
+        struct_valid P ->
+            forall (S : subst_ind),
+                (length (ptree_left P) = length S) ->
+                    In ((loop_head (ptree_constraint P) (ptree_left P) (ptree_right P) (ptree_deg P) bot), bot) (leaves P) ->
+                        In ((loop_head (ptree_constraint P) (batch_sub (ptree_left P) (univ v A) A S) (ptree_right P) (ptree_deg P) bot), bot) (leaves (ptree_ug_l_inv P A v S)).
+Proof.
+intros P A v.
+induction P;
+try intros PSV S EQ INPL;
+unfold ptree_ug_l_inv;
+unfold ug_left_inv_batch, batch_sub.
+
+1-3 : destruct PSV.
 5-11 : destruct PSV as [[[[[PSV [PG_app PD_app]] PG] PD] POC] PDeg].
 12 : destruct PSV as [[[[[[[PSV [PG_app PD_app]] PG] PD] KNING] KNIND] [KIN POC]] PDeg].
 13-14 : destruct PSV as [[[[[PSV [PG_app PD_app]] PG] PD] POC] PDeg].
@@ -338,10 +464,34 @@ unfold ug_left_inv_batch, batch_sub.
 17 : destruct PSV as [[[[[[[[[[P1SV P2SV] [PG_app PD_app]] P1G] P1D] P1OC] P2G] P2D] P2OC] PDeg1] PDeg2].
 18 : destruct PSV as [[[[[PSV [PG_app PD_app]] PG] PD] POC] PDeg].
 19 : destruct PSV as [[[[[[[[[[P1SV P2SV] [PG_app PD_app]] P1G] P1D] P1OC] P2G] P2D] P2OC] PDeg1] PDeg2].
+4 : destruct PSV as [[PSV [PG_app PD_app]] [PBot | [[[[[PRec PG] PD] POC] PDeg] PLoop]]].
 
-all : subst; 
+1-3 : inversion INPL as [].
+
+1 : { subst.
+      unfold ptree_constraint, ptree_left, ptree_right, ptree_deg in *.
+      rewrite EQ, nat_eqb_refl.
+      unfold ptree_ug_l_inv_fit, leaves.
+      rewrite batch_sub_fit_true.
+      apply (or_introl eq_refl).
+      rewrite EQ.
+      apply nat_eqb_refl. }
+
+1 : { inversion INPL as [INPL' | FAL];
+      try inversion FAL.
+      unfold ptree_constraint, ptree_left, ptree_right, ptree_deg in INPL';
+      fold ptree_constraint ptree_left ptree_right ptree_deg in *.
+      inversion INPL' as [[EQ1 EQ2]].
+      subst.
+      contradiction PRec. }
+
+
+
+all : subst;
+      try rewrite EQ, nat_eqb_refl.
+
       case nat_eqb eqn:EQ;
-      try reflexivity;
+      try apply INPL.
       unfold ptree_ug_l_inv_fit;
       fold ptree_ug_l_inv_fit;
       unfold ptree_left in EQ;
@@ -367,76 +517,27 @@ all : subst;
   rewrite PG.
   apply EQ.
 Qed.
-
-Lemma ug_l_formula_inv_vars :
-    forall (phi : formula) (A : formula) (v : ivar),
-        forall (b : bool),
-            vars_in (ug_left_inv_formula phi A v b) =
-                vars_in phi.
-Proof.
-intros phi A v b.
-unfold ug_left_inv_formula, formula_sub.
-case form_eqb eqn:EQf.
-case b.
-apply form_eqb_eq in EQf.
-subst.
-all : reflexivity.
-Qed.
-
-Lemma ptree_ug_l_inv_vars :
-    forall (gamma : list formula) (A : formula) (v : ivar),
-        forall (S : subst_ind),
-            flat_map vars_in (ug_left_inv_batch gamma A v S) =
-                flat_map vars_in gamma.
-Proof.
-induction gamma;
-intros A v S;
-unfold ug_left_inv_batch, batch_sub, batch_sub_fit;
-fold batch_sub_fit;
-destruct S;
-unfold length, nat_eqb;
-fold (@length formula) (@length bool) nat_eqb.
-1-3 : reflexivity.
-case nat_eqb eqn:EQn.
-unfold flat_map;
-fold (flat_map vars_in).
-rewrite (batch_sub_fit_true EQn).
-fold (ug_left_inv_batch gamma A v S).
-rewrite IHgamma.
-unfold formula_sub.
-case form_eqb eqn:EQf.
-case b.
-apply form_eqb_eq in EQf.
-subst.
-all : reflexivity.
-Qed.
-
-Lemma ptree_ug_l_inv_bot :
-    forall (phi : formula) (v : ivar) (S : subst_ind),
-        ptree_ug_l_inv bot phi v S = bot.
-Proof.
-intros phi v S.
-unfold ptree_ug_l_inv, ptree_ug_l_inv_fit.
-case (nat_eqb);
-reflexivity.
-Qed.
+*)
 
 Lemma ptree_ug_l_inv_struct :
     forall (P : ptree) (A : formula) (v : ivar),
         struct_valid P ->
-            forall (S : subst_ind),
-                struct_valid (ptree_ug_l_inv P A v S).
+            weak_formula A = false ->
+                forall (S : subst_ind),
+                    struct_valid (ptree_ug_l_inv P A v S).
 Proof.
 intros P.
 induction P;
-try intros AF vf PSV S;
+try intros AF vf PSV WF S;
 unfold ptree_ug_l_inv;
 unfold ug_left_inv_batch, batch_sub;
 case nat_eqb eqn:EQ;
-try apply PSV.
+try apply PSV;
+unfold ptree_ug_l_inv_fit;
+fold ptree_ug_l_inv_fit.
 
-all : unfold ptree_ug_l_inv_fit;
-      fold ptree_ug_l_inv_fit.
+16 :  destruct S as [ | b S];
+      try apply PSV.
 
 14 :  destruct S as [ | b S];
       try apply PSV.
@@ -444,83 +545,103 @@ all : unfold ptree_ug_l_inv_fit;
 12 :  destruct S as [ | b S];
       try apply PSV.
 
-10 :  destruct S as [ | b S];
-      try apply PSV.
-
-7 : destruct S as [ | b S];
+9 : destruct S as [ | b S];
     try apply PSV.
 
-2 : destruct S as [ | b1 [ | b2 S]];
+5 : destruct S as [ | b S];
     try apply PSV.
 
-1 : destruct PSV as [[[[[PSV [PG_app PD_app]] PL_OC] sig_C] [SUBG SUBD]] PLoop].
-2-8 : destruct PSV as [[[[[PSV [PG_app PD_app]] PG] PD] POC] PDeg].
-9 : destruct PSV as [[[[[[[PSV [PG_app PD_app]] PG] PD] KNING] KNIND] [KIN POC]] PDeg].
-10-11 : destruct PSV as [[[[[PSV [PG_app PD_app]] PG] PD] POC] PDeg].
-12 : destruct PSV as [[[[[[PSV [PG_app PD_app]] PG] PD] POC] POC_rel] PDeg].
-13 : destruct PSV as [[[[[[PSV [PG_app PD_app]] PG] PD] FRESH] [NING NIND]] PDeg].
-14 : destruct PSV as [[[[[[[[[[P1SV P2SV] [PG_app PD_app]] P1G] P1D] P1OC] P2G] P2D] P2OC] PDeg1] PDeg2].
-15 : destruct PSV as [[[[[PSV [PG_app PD_app]] PG] PD] POC] PDeg].
-16 : destruct PSV as [[[[[[[[[[P1SV P2SV] [PG_app PD_app]] P1G] P1D] P1OC] P2G] P2D] P2OC] PDeg1] PDeg2].
+4 : destruct S as [ | b1 [ | b2 S]];
+    try apply PSV.
+
+2 : destruct S as [ | b S];
+    try apply PSV.
+
+1 : destruct PSV as [[[PSV [PG_app PD_app]] [PBot | [[[[PRec PG] PD] POC] PDeg]]] PWF].
+3-9 : destruct PSV as [[[[[PSV [PG_app PD_app]] PG] PD] POC] PDeg].
+10-11 : destruct PSV as [[[[[[PSV [PG_app PD_app]] PG] PD] POC] PDeg] PWF].
+12 : destruct PSV as [[[[[[[PSV [PG_app PD_app]] PG] PD] KNING] KNIND] [KIN POC]] PDeg].
+13-14 : destruct PSV as [[[[[PSV [PG_app PD_app]] PG] PD] POC] PDeg].
+15 : destruct PSV as [[[[[[PSV [PG_app PD_app]] PG] PD] POC] POC_rel] PDeg].
+16 : destruct PSV as [[[[[[PSV [PG_app PD_app]] PG] PD] POC] [NING NIND]] PDeg].
+17 : destruct PSV as [[[[[[[[[[P1SV P2SV] [PG_app PD_app]] P1G] P1D] P1OC] P2G] P2D] P2OC] PDeg1] PDeg2].
+18 : destruct PSV as [[[[[PSV [PG_app PD_app]] PG] PD] POC] PDeg].
+19 : destruct PSV as [[[[[[[[[[P1SV P2SV] [PG_app PD_app]] P1G] P1D] P1OC] P2G] P2D] P2OC] PDeg1] PDeg2].
 
 all : subst.
 
-10 :  case (nat_eqb v vf && form_eqb phi AF) eqn:EQfn;
+13 :  case (nat_eqb v vf && form_eqb phi AF) eqn:EQfn;
       case b.
 
-1 : { destruct sig_C as [[[OC_Inj OC_Sur] Order] Coherent].
-      rewrite ptree_ug_l_inv_fit_true.
-      2 : { rewrite sublist_count_length, sublist_filter_true, map_length.
-            apply nat_eqb_refl.
-            apply SUBG.
-            rewrite sublist_filter_length.
-            apply (eq_sym (nat_eqb_eq _ _ EQ)).
-            apply SUBG. }
-      repeat split;
-      try rewrite P1G;
-      try rewrite P2G;
-      try apply EQ;
-      try unfold ptree_left at 1 in EQ;
-      try rewrite bury_length, <- (@bury_unbury _ S n), bury_length in EQ;
-      try apply EQ;
-      repeat split;
-      try rewrite ptree_ug_l_inv_constraint;
-      try apply ptree_ug_l_inv_deg;
-      try rewrite ptree_ug_l_inv_left;
-      try rewrite PG;
-      try rewrite P1G;
-      try rewrite P2G;
-      unfold flat_map;
-      fold (flat_map vars_in);
-      try rewrite ptree_ug_l_inv_vars;
-      try rewrite ug_l_formula_inv_vars;
-      unfold ug_left_inv_batch;
-      try rewrite batch_sub_false_head;
-      try rewrite ptree_ug_l_inv_right;
-      try apply Order;
-      try assumption;
-      try apply (IHP _ _ PSV);
-      try apply (IHP1 _ _ P1SV);
-      try apply (IHP2 _ _ P2SV);
-      try reflexivity.
-      - destruct PL_OC as [EQ' | PL_OC].
-        subst.
-        left.
-        apply ptree_ug_l_inv_bot.
+2 : { rewrite ptree_ug_l_inv_fit_true.
+      2 : apply EQ.
+      enough (struct_valid (loop_head (ptree_constraint P) (ug_left_inv_batch (ptree_left P) AF vf S) (ptree_right P) (ptree_deg P) (ptree_ug_l_inv P AF vf S))) as PSV'.
+      destruct P;
+      try apply PSV';
+      contradiction (PRec eq_refl).
+      repeat split.
+      - apply (IHP _ _ PSV WF).
+      - rewrite ptree_ug_l_inv_vars.
+        apply PG_app.
+        apply WF.
+      - apply PD_app.
+      - destruct (ptree_eq_dec (ptree_ug_l_inv P AF vf S) bot) as [EQ' | NE].
+        apply (inl EQ').
         right.
-        apply PL_OC.
-      - pose proof (batch_sub_sublist _ _ (univ vf AF) AF S SUBG (nat_eqb_eq _ _ EQ)).
-        rewrite map_batch_sub.
-        + admit.
-        + intros phi1 phi2.
-          split;
-          intros EQ'.
-          subst.
-          reflexivity.
-          
-          admit.
-      - admit.
-}
+        repeat split;
+        try rewrite P1G;
+        try rewrite P2G;
+        try apply EQ;
+        try unfold ptree_left at 1 in EQ;
+        try rewrite bury_length, <- (@bury_unbury _ S n), bury_length in EQ;
+        try apply EQ;
+        repeat split;
+        try rewrite ptree_ug_l_inv_constraint;
+        try apply ptree_ug_l_inv_deg;
+        try rewrite ptree_ug_l_inv_left;
+        try rewrite PG;
+        try rewrite P1G;
+        try rewrite P2G;
+        unfold flat_map;
+        fold (flat_map vars_in);
+        try rewrite ptree_ug_l_inv_vars;
+        try rewrite ug_l_formula_inv_vars;
+        unfold ug_left_inv_batch;
+        try rewrite batch_sub_false_head;
+        try rewrite ptree_ug_l_inv_right;
+        try apply Order;
+        try assumption;
+        try apply (IHP _ _ PSV);
+        try apply (IHP1 _ _ P1SV);
+        try apply (IHP2 _ _ P2SV);
+        try reflexivity.
+      - intros phi [INL | INR].
+        + unfold ug_left_inv_batch in INL.
+          rewrite batch_sub_is_map_combine in INL.
+          apply in_map_iff in INL as [[psi b] [EQF IN]].
+          apply in_combine_l in IN.
+          rewrite <- EQF.
+          unfold fst, snd.
+          refine (not_weak_sub_not_weak _ _ _ (PWF _ (or_introl IN)) WF _).
+          apply nat_eqb_eq, EQ.
+        + apply (PWF _ (or_intror INR)). }
+
+1 : { repeat split.
+      rewrite ptree_ug_l_inv_vars.
+      apply PG_app.
+      apply WF.
+      apply PD_app.
+      apply (inl eq_refl).
+      intros phi [INL | INR].
+      - unfold ug_left_inv_batch in INL.
+        rewrite batch_sub_is_map_combine in INL.
+        apply in_map_iff in INL as [[psi b] [EQF IN]].
+        apply in_combine_l in IN.
+        rewrite <- EQF.
+        unfold fst, snd.
+        refine (not_weak_sub_not_weak _ _ _ (PWF _ (or_introl IN)) WF _).
+        apply nat_eqb_eq, EQ.        
+      - apply (PWF _ (or_intror INR)). }
 
 all : repeat rewrite ptree_ug_l_inv_fit_true;
       try rewrite PG;
@@ -545,169 +666,20 @@ all : repeat rewrite ptree_ug_l_inv_fit_true;
       try rewrite batch_sub_false_head;
       try rewrite ptree_ug_l_inv_right;
       try assumption;
-      try apply (IHP _ _ PSV);
-      try apply (IHP1 _ _ P1SV);
-      try apply (IHP2 _ _ P2SV);
+      try apply (IHP _ _ PSV WF);
+      try apply (IHP1 _ _ P1SV WF);
+      try apply (IHP2 _ _ P2SV WF);
       try reflexivity.
 
-1 : unfold batch_sub, batch_sub_fit;
-    fold batch_sub_fit.
-    unfold length in *;
-    fold (@length formula) (@length bool) in *;
-    unfold nat_eqb in *;
-    fold nat_eqb in *.
-    rewrite EQ.
-    unfold formula_sub at 1, form_eqb, ug_left_inv_formula.
-    admit.
-Qed.
-
-Lemma demorgan1_valid :
-    forall (P : ptree) (E F : formula),
-        valid P ->
-            forall (S : subst_ind),
-                subst_ind_fit (ptree_formula P) S = true ->
-                    valid (demorgan1_sub_ptree P E F S).
-Proof.
-intros P E F [PSV PAX].
-induction P; try intros S FS;
-unfold demorgan1_sub_ptree;
-rewrite FS;
-unfold ptree_formula in *; fold ptree_formula in *;
-unfold demorgan1_sub_ptree_fit; fold demorgan1_sub_ptree_fit.
-
-all : try apply (PSV,PAX).
-
-1 : { repeat split.
-      rewrite dem1_axiom_id;
-      apply PAX.
-      apply or_introl, eq_refl. }
-
-  1 : destruct PSV as [PSV DU].
-  2 : destruct PSV as [[PSV OU] NO].
-  3-10 : destruct PSV as [[[PF PSV] PD] PO].
-  11 : destruct PSV as [[[[PF PSV] PD] PO] FC].
-  12-16: destruct PSV as [[[[[[[P1F P1SV] P1D] P1O] P2F] P2SV] P2D] P2O].
-  17: destruct PSV as [[[[[[[[P1F P1SV] P1D] P1O] P2F] P2SV] P2D] P2O] INA].
-
-  3-6,8-13,16,17 : 
-      destruct S; inversion FS as [FS'];
-      try destruct (and_bool_prop _ _ FS') as [FS1 FS2].
-
-  4-6,13 :  destruct S1; inversion FS' as [FS''];
-            try destruct (and_bool_prop _ _ FS1) as [FS1_1 FS1_2].
-
-  6 : destruct S1_1; inversion FS'' as [FS'''];
-      destruct (and_bool_prop _ _ FS1_1) as [FS1_1_1 FS1_1_2].
-
-  7,8,13,14 :
-      case (form_eqb a E) eqn:EQ1;
-      case (form_eqb b F) eqn:EQ2;
-      unfold ptree_deg; fold ptree_deg;
-      try apply (PSV,PAX).
-
-11,19 : case (nat_eqb d1 (Nat.max d1 d2)) eqn:EQ.
-
-
-all : unfold node_extract in *;
-      fold node_extract in *;
-      try apply form_eqb_eq in EQ1;
-      try destruct EQ1;
-      try apply form_eqb_eq in EQ2;
-      try destruct EQ2;
-      repeat rewrite demorgan1_ptree_formula_true;
-      repeat split;
-      try apply IHP;
-      try apply (IHP1 P1SV);
-      try apply (IHP2 P2SV);
-      unfold ptree_deg; fold ptree_deg;
-      try rewrite demorgan1_ptree_deg;
-      try rewrite demorgan1_ptree_ord;
-      try apply ptree_ord_nf_struct;
-      unfold ptree_ord; fold ptree_ord;
-      try rewrite demorgan1_ptree_formula;
-      try rewrite PF;
-      try rewrite P1F;
-      try rewrite P2F;
-      repeat split;
-      unfold demorgan1_sub_formula;
-      repeat rewrite formula_sub_ind_lor;
-      try rewrite formula_sub_ind_0;
-      try rewrite non_target_sub;
-      try rewrite non_target_sub_term;
-      try apply PSV;
-      try apply PAX;
-      try apply PD;
-      try rewrite PO;
-      try apply P1SV;
-      try rewrite P1D in *;
-      try rewrite P1O;
-      try apply P2SV;
-      try rewrite P2D in *;
-      try rewrite P2O;
-      try apply FS;
-      try apply DU;
-      try apply OU;
-      try apply NO;
-      try apply INA;
-      try rewrite PF;
-      try rewrite P1F;
-      try rewrite P2F;
-      unfold subst_ind_fit, non_target;
-      fold subst_ind_fit non_target;
-      try rewrite non_target_fit;
-      try rewrite non_target_sub_fit;
-      try rewrite FS;
-      try rewrite FS';
-      try rewrite FS'';
-      try rewrite FS1;
-      try rewrite FS1_1;
-      try rewrite FS1_2;
-      try rewrite FS1_1_1;
-      try rewrite FS1_1_2;
-      try rewrite FS2;
-      unfold "&&";
+all : try rewrite <- batch_sub_fit_true;
+      unfold batch_sub_fit;
+      fold batch_sub_fit;
+      try rewrite batch_sub_fit_true;
       try reflexivity;
-      try apply (fun B INB => PAX B (in_or_app _ _ _ (or_introl INB)));
-      try apply (fun B INB => PAX B (in_or_app _ _ _ (or_intror INB)));
-      try apply max_lem1;
-      try apply EQ;
-      try apply ord_lt_max_succ_l;
-      try reflexivity.
+      try apply EQ.
 
-  8 : { intros B INB.
-        rewrite closed_free_list in INB.
-        inversion INB.
-        apply formula_sub_ind_closed.
-        apply (valid_closed_formula PAX FC).
-        intros CEF.
-        apply and_bool_prop in CEF as [CE CF].
-        apply CE. }
+1 : rewrite <- (form_sub_sub0_comm _ _ _ _ _ WF).
+    reflexivity.
 
-  all : unfold node_extract in *;
-        fold node_extract in *;
-        intros A IN;
-        try apply in_app_or in IN as [IN1 | IN2];
-        try apply (fun FSUB => dem1_all_ax_trans _ _ _ _ P1SV FSUB (fun B INB1 => PAX B (in_or_app _ _ _ (or_introl INB1))) _ IN1);
-        try apply (fun FSUB => dem1_all_ax_trans _ _ _ _ P2SV FSUB (fun B INB2 => PAX B (in_or_app _ _ _ (or_intror INB2))) _ IN2);
-        try apply (PAX _ (in_or_app _ _ _ (or_introl IN1)));
-        try apply (PAX _ (in_or_app _ _ _ (or_intror IN2)));
-        try rewrite P1F;
-        try rewrite P2F;
-        unfold subst_ind_fit;
-        fold subst_ind_fit;
-        try rewrite FS;
-        try rewrite FS1;
-        try rewrite FS2;
-        try rewrite non_target_fit;
-        try reflexivity.
-
-  all : try apply (PAX _ (in_or_app _ _ _ (or_intror IN)));
-        try apply in_app_or in IN as [IN1 | IN2];
-        try apply (PAX _ (in_or_app _ _ _ (or_introl IN1)));
-        try apply (fun FSUB => dem1_all_ax_trans _ _ _ _ P1SV FSUB (fun B INB => PAX B (in_or_app _ _ _ (or_intror INB))) _ IN2);
-        try rewrite P1F;
-        unfold subst_ind_fit;
-        fold subst_ind_fit;
-        try rewrite FS1, non_target_sub_fit;
-        try reflexivity.
+1 : apply (not_weak_sub_not_weak _ _ _ PWF WF).
 Qed.
